Flushing out a small amount of the proof structure

stanfrontend/CStan.v
@@ -585,13 +585,13 @@ Inductive initial_state_gen (p: program) (m: mem) (i: ident): state -> Prop :=
       type_of_fundef f = Tfunction Tnil Tvoid cc_default ->
       initial_state_gen p m i (Callstate f nil Kstop m zero).						      
 
-Inductive final_state_gen: state -> int -> Prop :=
+Inductive final_state: state -> int -> Prop :=
   | final_state_data_intro: forall r m ta,
-      final_state_gen (Returnstate (Vint r) Kstop m ta) r.
+      final_state (Returnstate (Vint r) Kstop m ta) r.
 
 Definition semantics_gen (p: program) (m: mem) (i: ident) :=
   let ge := globalenv p in
-  Semantics_gen stepf (initial_state_gen p m i) final_state_gen ge ge.
+  Semantics_gen stepf (initial_state_gen p m i) final_state ge ge.
 
 Definition semantics_data (p: program) (m: mem) :=
   semantics_gen p m p.(prog_data).
@@ -607,6 +607,9 @@ Definition semantics_transformed_parameters (p: program) (m: mem) :=
 						      
 Definition semantics_generated_quantities (p: program) (m: mem) :=
   semantics_gen p m p.(prog_generated_quantities).
+
+Definition initial_state (p: program) (m: mem) :=
+  initial_state_gen p m p.(prog_model).
 
 Definition semantics (p: program) (m: mem) :=
   semantics_gen p m p.(prog_model).
