stanfrontend/Sbackendproof.v
@@ -18,11 +18,39 @@ Hypothesis INITMEM: Genv.init_mem prog = Some m0.
 Let ge := CStan.globalenv prog.
 Let tge := globalenv tprog.
 
-Check Clight.semantics1.
-Check CStan.semantics.
+Variable match_states: CStan.state -> Clight.state -> Prop. 
+
+Lemma senv_preserved: Senv.equiv ge tge.
+Proof.
+Admitted.
+
+Lemma step_simulation:
+  forall S1 t S2, CStan.stepf ge S1 t S2 ->
+  forall S1' (MS: match_states S1 S1'), exists S2', plus Clight.step1 tge S1' t S2' /\ match_states S2 S2'.
+Proof.
+Admitted.
+
+Lemma initial_states_simulation:
+  forall S, CStan.initial_state prog m0 S ->
+  exists R, Clight.initial_state tprog R /\ match_states S R.
+Proof.
+Admitted.
+
+Lemma final_states_simulation:
+  forall S R r,
+  match_states S R -> CStan.final_state S r -> Clight.final_state R r.
+Proof.
+Admitted.
+
 
 Theorem transf_program_correct:
   forward_simulation (CStan.semantics prog m0) (Clight.semantics1 tprog).
+Proof.
+  eapply forward_simulation_plus.
+  apply senv_preserved.
+  eexact initial_states_simulation.
+  eexact final_states_simulation.
+  eexact step_simulation.
 Admitted.
 
 End PRESERVATION.
